plugins/syntax/string_notation.ml
@@ -1,0 +1,97 @@
+(************************************************************************)
+(*         *   The Coq Proof Assistant / The Coq Development Team       *)
+(*  v      *   INRIA, CNRS and contributors - Copyright 1999-2018       *)
+(* <O___,, *       (see CREDITS file for the list of authors)           *)
+(*   \VV/  **************************************************************)
+(*    //   *    This file is distributed under the terms of the         *)
+(*         *     GNU Lesser General Public License Version 2.1          *)
+(*         *     (see LICENSE file for the text of the license)         *)
+(************************************************************************)
+
+open Pp
+open Util
+open Names
+open Libnames
+open Globnames
+open Constrexpr
+open Constrexpr_ops
+open Notation
+
+(** * String notation *)
+
+let get_constructors ind =
+  let mib,oib = Global.lookup_inductive ind in
+  let mc = oib.Declarations.mind_consnames in
+  Array.to_list
+    (Array.mapi (fun j c -> ConstructRef (ind, j + 1)) mc)
+
+let qualid_of_ref n =
+  n |> Coqlib.lib_ref |> Nametab.shortest_qualid_of_global Id.Set.empty
+
+let q_option () = qualid_of_ref "core.option.type"
+let q_list () = qualid_of_ref "core.list.type"
+let q_byte () = qualid_of_ref "core.byte.type"
+
+let has_type f ty =
+  let (sigma, env) = Pfedit.get_current_context () in
+  let c = mkCastC (mkRefC f, Glob_term.CastConv ty) in
+  try let _ = Constrintern.interp_constr env sigma c in true
+  with Pretype_errors.PretypeError _ -> false
+
+let type_error_to f ty =
+  CErrors.user_err
+    (pr_qualid f ++ str " should go from Byte.byte or (list Byte.byte) to " ++
+     pr_qualid ty ++ str " or (option " ++ pr_qualid ty ++ str ").")
+
+let type_error_of g ty =
+  CErrors.user_err
+    (pr_qualid g ++ str " should go from " ++ pr_qualid ty ++
+     str " to Byte.byte or (option Byte.byte) or (list Byte.byte) or (option (list Byte.byte)).")
+
+let vernac_string_notation local ty f g scope =
+  let app x y = mkAppC (x,[y]) in
+  let cref q = mkRefC q in
+  let cbyte = cref (q_byte ()) in
+  let clist = cref (q_list ()) in
+  let coption = cref (q_option ()) in
+  let opt r = app coption r in
+  let clist_byte = app clist cbyte in
+  let tyc = Smartlocate.global_inductive_with_alias ty in
+  let to_ty = Smartlocate.global_with_alias f in
+  let of_ty = Smartlocate.global_with_alias g in
+  let cty = cref ty in
+  let arrow x y =
+    mkProdC ([CAst.make Anonymous],Default Decl_kinds.Explicit, x, y)
+  in
+  let constructors = get_constructors tyc in
+  (* Check the type of f *)
+  let to_kind =
+    if has_type f (arrow clist_byte cty) then ListByte, Direct
+    else if has_type f (arrow clist_byte (opt cty)) then ListByte, Option
+    else if has_type f (arrow cbyte cty) then Byte, Direct
+    else if has_type f (arrow cbyte (opt cty)) then Byte, Option
+    else type_error_to f ty
+  in
+  (* Check the type of g *)
+  let of_kind =
+    if has_type g (arrow cty clist_byte) then ListByte, Direct
+    else if has_type g (arrow cty (opt clist_byte)) then ListByte, Option
+    else if has_type g (arrow cty cbyte) then Byte, Direct
+    else if has_type g (arrow cty (opt cbyte)) then Byte, Option
+    else type_error_of g ty
+  in
+  let o = { sto_kind = to_kind;
+            sto_ty = to_ty;
+            sof_kind = of_kind;
+            sof_ty = of_ty;
+            string_ty = ty }
+  in
+  let i =
+       { pt_local = local;
+         pt_scope = scope;
+         pt_interp_info = StringNotation o;
+         pt_required = Nametab.path_of_global (IndRef tyc),[];
+         pt_refs = constructors;
+         pt_in_match = true }
+  in
+  enable_prim_token_interpretation i
