vernac/himsg.ml
@@ -1326,12 +1326,12 @@ let explain_reduction_tactic_error = function
       spc () ++ str "is not well typed." ++ fnl () ++
       explain_type_error env' (Evd.from_env env') e
 
-let explain_numeral_notation_error env sigma = function
+let explain_numeral_or_string_notation_error numeral_or_string env sigma = function
   | Notation.UnexpectedTerm c ->
     (strbrk "Unexpected term " ++
      pr_constr_env env sigma c ++
-     strbrk " while parsing a numeral notation.")
+     strbrk (" while parsing a "^numeral_or_string^" notation."))
   | Notation.UnexpectedNonOptionTerm c ->
     (strbrk "Unexpected non-option term " ++
      pr_constr_env env sigma c ++
-     strbrk " while parsing a numeral notation.")
+     strbrk (" while parsing a "^numeral_or_string^" notation."))
