test-suite/output/StringSyntax.v
@@ -1,0 +1,39 @@
+Require Import Coq.Lists.List.
+Require Import Coq.Strings.String Coq.Strings.Byte Coq.Strings.Ascii.
+Import ListNotations.
+
+Set Printing Depth 100000.
+Set Printing Width 1000.
+
+Close Scope char_scope.
+Close Scope string_scope.
+
+Open Scope byte_scope.
+Print byte_rect.
+Print byte_rec.
+Print byte_ind.
+Check "000".
+Check "a".
+Check "127".
+Fail Check "€".
+Close Scope byte_scope.
+
+Open Scope char_scope.
+Check "000".
+Check "a".
+Check "127".
+Fail Check "€".
+Close Scope char_scope.
+
+Open Scope string_scope.
+Check "000".
+Check "a".
+Check "127".
+Check "€".
+Check String "001" EmptyString.
+Close Scope string_scope.
+
+Compute ascii_of_byte "a".
+Compute byte_of_ascii "a".
+Compute string_of_list_byte ("a"::nil)%byte.
+Compute list_byte_of_string "a".
